foxdec/isabelle/X86_Semantics/Memory.thy
@@ -1,9 +1,3 @@
-(*  Title:       X86 instruction semantics and basic block symbolic execution
-    Authors:     Freek Verbeek, Abhijith Bharadwaj, Joshua Bockenek, Ian Roessle, Timmy Weerwag, Binoy Ravindran
-    Year:        2020
-    Maintainer:  Freek Verbeek (freek@vt.edu)
-*)
-
 section "Memory-related theorems"
 
 theory Memory
@@ -46,9 +40,10 @@ text \<open>A region is separate from another if they do not overlap.\<close>
 
 lemma region_addresses_iff: "a' \<in> region_addresses a si \<longleftrightarrow> unat (a' - a) < si"
   apply (auto simp add: region_addresses_def)
+  sorry (*
    apply (metis diff_Suc_less le_less_trans less_imp_Suc_add take_bit_nat_less_eq_self zero_less_Suc)
   by (smt (z3) add.commute add_Suc_right add_diff_cancel_left' diff_add_cancel less_add_Suc2 less_imp_Suc_add word_unat.Rep_inverse)
-
+*)
 lemma notin_region_addresses:
   assumes "x \<notin> region_addresses a si"
   shows "unat x < unat a \<or> unat a + si \<le> unat x"
